test/KMS/Integration.dfy
@@ -1,0 +1,91 @@
+// RUN: %dafny /out:Output/Integration.exe "./Integration.dfy" ../../src/extern/dotnet/KMS.cs ../../src/extern/dotnet/UTF8.cs ../../src/extern/dotnet/Arrays-extern.cs ../../src/extern/dotnet/HKDF-extern.cs ../../src/extern/dotnet/AESEncryption.cs ../../src/extern/dotnet/Random.cs ../../src/extern/dotnet/Signature.cs "%kmslib" "%awslib" "%bclib" /compile:2
+// RUN: cp %awslib %kmslib %bclib Output/
+// RUN: %mono ./Output/Integration.exe > "%t"
+// RUN: %diff "%s.expect" "%t"
+
+include "../../src/SDK/Keyring/KMSKeyring.dfy"
+include "../../src/SDK/Materials.dfy"
+include "../../src/StandardLibrary/StandardLibrary.dfy"
+include "../../src/StandardLibrary/UInt.dfy"
+include "../../src/SDK/CMM/Defs.dfy"
+include "../../src/SDK/CMM/DefaultCMM.dfy"
+include "../../src/SDK/Client.dfy"
+include "../../src/SDK/MessageHeader.dfy"
+include "../../src/KMS/KMSUtils.dfy"
+include "../../src/Util/UTF8.dfy"
+include "../../src/StandardLibrary/Base64.dfy"
+
+module IntegTestKMS {
+  import opened StandardLibrary
+  import opened UInt = StandardLibrary.UInt
+  import CMMDefs
+  import DefaultCMMDef
+  import KMSUtils
+  import KMSKeyring
+  import Materials
+  import Client = ESDKClient
+  import Msg = MessageHeader
+  import UTF8
+  import Base64
+
+  method EncryptDecryptTest(cmm: CMMDefs.CMM, message: string) returns (res: Result<string>)
+    requires cmm.Valid()
+  {
+    var encodedMsg: seq<uint8>;
+    var encodeResult := UTF8.Encode(message);
+    if encodeResult.Success? {
+      encodedMsg := encodeResult.value;
+    }
+    var keyA, valA := UTF8.Encode("keyA").value, UTF8.Encode("valA").value;
+    var encryptionContext := [(keyA, valA)];
+    assert Msg.ValidAAD(encryptionContext) by {
+      // To proving ValidAAD, we need to reveal the definition of ValidAAD:
+      reveal Msg.ValidAAD();
+      // We also need to help the verifier with proving the AADLength is small:
+      calc {
+        Msg.AADLength(encryptionContext);
+        2 + Msg.KVPairsLength(encryptionContext, 0, 1);
+        2 + 2 + |keyA| + 2 + |valA|;
+      }
+      assert Msg.AADLength(encryptionContext) < UINT16_LIMIT;
+    }
+    var e := Client.Encrypt(encodedMsg, cmm, encryptionContext);
+    if e.Failure? {
+      return Failure("Bad encryption :( " + e.error + "\n");
+    }
+
+    var d := Client.Decrypt(e.value, cmm);
+    if d.Failure? {
+      return Failure("bad decryption: " + d.error + "\n");
+    }
+    if UTF8.ValidUTF8Seq(d.value) {
+      return UTF8.Decode(d.value);
+    } else {
+      return Failure("Could not decode Encryption output");
+    }
+  }
+
+  method Main() {
+    var namespace := UTF8.Encode("namespace");
+    var name := UTF8.Encode("MyKeyring");
+    if name.Failure? || namespace.Failure? {
+      print "Failure: hardcoded name/namespace cannot be utf8 encoded";
+      return;
+    }
+
+    var generator := "arn:aws:kms:us-west-2:658956600833:key/b3537ef1-d8dc-4780-9f5a-55776cbb2f7f";
+    var clientSupplier := new KMSUtils.DefaultClientSupplier();
+    var keyring := new KMSKeyring.KMSKeyring(clientSupplier, [], Some(generator), []);
+    var cmm := new DefaultCMMDef.DefaultCMM.OfKeyring(keyring);
+
+    var message := "Hello, World!";
+
+    var result := EncryptDecryptTest(cmm, message);
+
+    if result.Success? && result.value == message {
+      print "CORRECT\n";
+    } else {
+      print "NOT CORRECT\n";
+    }
+  }
+}
